cQp algebra

theories/lang/cpp/logic/heap_pred.v
@@ -17,6 +17,7 @@ From bedrock.lang.cpp Require Import
 
 Export bedrock.lang.cpp.logic.rep.
 Export bedrock.lang.cpp.heap_notations.
+Export bedrock.lang.algebra.cqp.
 
 Implicit Types (σ resolve : genv) (p : ptr) (o : offset).
 
@@ -25,7 +26,7 @@ Section defs.
 
   (** object identity *)
   Definition identityR {σ : genv} (cls : globname) (mdc : list globname)
-             (q : Qp) : Rep :=
+             (q : cQp) : Rep :=
     as_Rep (@identity _ _ σ cls mdc q).
   (** cpp2v-core#194: [Fractional], [AsFractional], [Timeless]? *)
   (** cpp2v-core#194: The fraction is valid? Agreement? *)
@@ -61,7 +62,7 @@ Section with_cpp.
    *
    * NOTE [ty] *must* be a primitive type.
    *)
-  Definition primR_def {resolve:genv} (ty : type) (q : Qp) (v : val) : Rep :=
+  Definition primR_def {resolve:genv} (ty : type) (q : cQp) (v : val) : Rep :=
     as_Rep (fun addr => tptsto ty q addr v **
                       [| not(exists raw, v = Vraw raw) |] **
                       [| has_type v (drop_qualifiers ty) |]).
@@ -89,15 +90,31 @@ Section with_cpp.
     : Timeless (primR ty q v).
   Proof. rewrite primR_eq. apply _. Qed.
 
-  #[global] Instance primR_fractional resolve ty v :
-    Fractional (λ q, primR ty q v).
+  #[global] Instance primR_fractional resolve ty v q_c :
+    Fractional (λ q, primR ty (cqp.mk q_c q) v).
   Proof. rewrite primR_eq. apply _. Qed.
   #[global] Instance primR_as_fractional resolve ty q v :
-    AsFractional (primR ty q v) (λ q, primR ty q v) q.
+    AsFractional (primR ty q v) (λ q', primR ty (cqp.mk (is_const q) q') v) (frac q).
+  Proof. constructor. case: q=>>//=. apply _. Qed.
+
+  Parameter primR' : type → Qp → val → Rep.
+  Instance primR_fractional' resolve ty v :
+    Fractional (λ q, primR' ty q v).
+  Proof. Admitted.
+  #[global] Instance primR_as_fractional' resolve ty q v :
+    AsFractional (primR' ty q v) (λ q', primR' ty q' v) q.
   Proof. constructor. done. apply _. Qed.
 
-  #[global] Instance primR_observe_frac_valid resolve ty (q : Qp) v :
-    Observe [| q ≤ 1 |]%Qp (primR ty q v).
+  Lemma test1 T q v (p : ptr) : primR' T q v p |-- emp.
+  Proof.
+    iIntros "H".
+
+    iDestruct (as_fractional with "H") as "?".
+    iDestructHyp "H" as "[??]".
+         
+  
+  #[global] Instance primR_observe_frac_valid resolve ty (q : cQp) v :
+    Observe [| cqp.frac q ≤ 1 |]%Qp (primR ty q v).
   Proof. rewrite primR_eq. apply _. Qed.
 
   #[global] Instance primR_observe_agree resolve ty q1 q2 v1 v2 :
@@ -140,7 +157,7 @@ Section with_cpp.
      TODO is it possible to generalize this to support aggregate types? structures seem easy enough
           but unions seem more difficult, possibly we can achieve that through the use of disjunction?
    *)
-  Definition uninitR_def {resolve:genv} (ty : type) (q : Qp) : Rep :=
+  Definition uninitR_def {resolve:genv} (ty : type) (q : cQp) : Rep :=
     as_Rep (fun addr => @tptsto _ _ resolve ty q addr Vundef).
   Definition uninitR_aux : seal (@uninitR_def). Proof. by eexists. Qed.
   Definition uninitR := uninitR_aux.(unseal).
@@ -164,15 +181,15 @@ Section with_cpp.
     : Timeless (uninitR ty q).
   Proof. rewrite uninitR_eq. apply _. Qed.
 
-  #[global] Instance uninitR_fractional resolve ty :
-    Fractional (uninitR ty).
+  #[global] Instance uninitR_fractional resolve ty c_q :
+    Fractional (fun q => uninitR ty (cqp.mk c_q q)).
   Proof. rewrite uninitR_eq. apply _. Qed.
-  #[global] Instance unintR_as_fractional resolve ty q :
-    AsFractional (uninitR ty q) (uninitR ty) q.
+  #[global] Instance unintR_as_fractional resolve ty c_q q :
+    AsFractional (uninitR ty (cqp.mk c_q q)) (fun q => uninitR ty (cqp.mk c_q q)) q.
   Proof. constructor. done. apply _. Qed.
 
-  #[global] Instance uninitR_observe_frac_valid resolve ty (q : Qp) :
-    Observe [| q ≤ 1 |]%Qp (uninitR ty q).
+  #[global] Instance uninitR_observe_frac_valid resolve ty (q : cQp) :
+    Observe [| cqp.frac q ≤ 1 |]%Qp (uninitR ty q).
   Proof. rewrite uninitR_eq. apply _. Qed.
 
   Lemma test:
@@ -186,10 +203,10 @@ Section with_cpp.
   Qed.
 
   (** This seems odd, but it's relevant to proof that [anyR] is fractional. *)
-  Lemma primR_uninitR {resolve} ty q1 q2 v :
-    primR ty q1 v |--
-    uninitR ty q2 -*
-    primR ty (q1 + q2) Vundef.
+  Lemma primR_uninitR {resolve} ty c_q q1 q2 v :
+    primR ty (cqp.mk c_q q1) v |--
+    uninitR ty (cqp.mk c_q q2) -*
+    primR ty (mk c_q (q1 + q2)) Vundef.
   Proof.
     rewrite primR_eq/primR_def uninitR_eq/uninitR_def. constructor=>p /=.
     rewrite monPred_at_wand. iIntros "[T1 [%Hnotraw %Hty]]" (? <-%ptr_rel_elim) "/= T2".
@@ -202,20 +219,20 @@ Section with_cpp.
 
   (** [anyR] The argument pointers points to a value of C++ type [ty] that might be
       uninitialized. *)
-  Parameter anyR : ∀ {resolve} (ty : type) (q : Qp), Rep.
+  Parameter anyR : ∀ {resolve} (ty : type) (q : cQp), Rep.
   #[global] Arguments anyR {resolve} ty q : rename.
   Axiom anyR_timeless : ∀ resolve ty q, Timeless (anyR ty q).
-  Axiom anyR_fractional : ∀ resolve ty, Fractional (anyR ty).
-  Axiom anyR_observe_frac_valid : ∀ resolve ty (q : Qp),
-    Observe [| q ≤ 1 |]%Qp (anyR ty q).
+  Axiom anyR_fractional : ∀ resolve ty c_q, Fractional (fun q => anyR ty (cqp.mk c_q q)).
+  Axiom anyR_observe_frac_valid : ∀ resolve ty (q : cQp),
+    Observe [| cqp.frac q ≤ 1 |]%Qp (anyR ty q).
   Axiom primR_anyR : ∀ resolve t q v, primR t q v |-- anyR t q.
   Axiom uninitR_anyR : ∀ resolve t q, uninitR t q |-- anyR t q.
   Axiom tptsto_raw_anyR : forall resolve p q r, tptsto Tu8 q p (Vraw r) |-- p |-> anyR Tu8 q.
   Axiom anyR_type_ptr_observe : ∀ σ ty q, Observe (type_ptrR ty) (anyR ty q).
 
   #[global] Existing Instances anyR_timeless anyR_fractional anyR_observe_frac_valid anyR_type_ptr_observe.
-  #[global] Instance anyR_as_fractional resolve ty q :
-    AsFractional (anyR ty q) (anyR ty) q.
+  #[global] Instance anyR_as_fractional resolve ty c_q q :
+    AsFractional (anyR ty (cqp.mk c_q q)) (fun q => anyR ty (cqp.mk c_q q)) q.
   Proof. exact: Build_AsFractional. Qed.
 
   Axiom _at_anyR_ptr_congP_transport : forall {σ} p p' ty q,
@@ -365,7 +382,7 @@ Section with_cpp.
 
   (** [blockR sz q] represents [q] ownership of a contiguous chunk of
       [sz] bytes without any C++ structure on top of it. *)
-  Definition blockR_def {σ} sz (q : Qp) : Rep :=
+  Definition blockR_def {σ} sz (q : cQp) : Rep :=
     _offsetR (o_sub σ Tu8 (Z.of_N sz)) validR **
     (* ^ Encodes valid_ptr (this .[ Tu8 ! sz]). This is
     necessary to get [l |-> blockR n -|- l |-> blockR n ** l .[ Tu8 ! m] |-> blockR 0]. *)
@@ -379,18 +396,18 @@ Section with_cpp.
   #[global] Instance blockR_timeless {resolve : genv} sz q :
     Timeless (blockR sz q).
   Proof. rewrite blockR_eq /blockR_def. unfold_at. apply _. Qed.
-  #[global] Instance blockR_fractional resolve sz :
-    Fractional (blockR sz).
+  #[global] Instance blockR_fractional resolve sz c_q :
+    Fractional (fun q => blockR sz (cqp.mk c_q q)).
   Proof.
     by rewrite blockR_eq /blockR_def; apply _.
   Qed.
-  #[global] Instance blockR_as_fractional resolve sz q :
-    AsFractional (blockR sz q) (blockR sz) q.
+  #[global] Instance blockR_as_fractional resolve sz c_q q :
+    AsFractional (blockR sz (mk c_q q)) (fun q => blockR sz (cqp.mk c_q q)) q.
   Proof. exact: Build_AsFractional. Qed.
 
-  #[global] Instance blockR_observe_frac_valid resolve sz (q : Qp) :
+  #[global] Instance blockR_observe_frac_valid resolve sz (q : cQp) :
     TCLt (0 ?= sz)%N ->
-    Observe [| q ≤ 1 |]%Qp (blockR sz q).
+    Observe [| cqp.frac q ≤ 1 |]%Qp (blockR sz q).
   Proof.
     rewrite TCLt_N blockR_eq/blockR_def. intros.
     destruct (N.to_nat sz) eqn:?; [ lia | ] => /=.
@@ -401,7 +418,7 @@ Section with_cpp.
    * it is a convenient short-hand since it happens frequently, but there is nothing
    * special about it.
    *)
-  Definition tblockR {σ} (ty : type) (q : Qp) : Rep :=
+  Definition tblockR {σ} (ty : type) (q : cQp) : Rep :=
     match size_of σ ty , align_of ty with
     | Some sz , Some al => blockR (σ:=σ) sz q ** alignedR al
     | _ , _  => False
@@ -410,25 +427,27 @@ Section with_cpp.
   #[global] Instance tblockR_timeless ty q :
     Timeless (tblockR ty q).
   Proof. rewrite/tblockR. case_match; apply _. Qed.
-  #[global] Instance tblockR_fractional ty :
-    Fractional (tblockR ty).
+  #[global] Instance tblockR_fractional ty c_q :
+    Fractional (fun q => tblockR ty (cqp.mk c_q q)).
   Proof.
     rewrite/tblockR. do 2!(case_match; last by apply _).
     apply _.
   Qed.
-  #[global] Instance tblockR_as_fractional ty q :
-    AsFractional (tblockR ty q) (tblockR ty) q.
+  #[global] Instance tblockR_as_fractional ty c_q q :
+    AsFractional (tblockR ty (cqp.mk c_q q)) (fun q => tblockR ty (cqp.mk c_q q)) q.
   Proof. exact: Build_AsFractional. Qed.
   #[global] Instance tblockR_observe_frac_valid ty q n :
     SizeOf ty n -> TCLt (0 ?= n)%N ->
-    Observe [| q ≤ 1 |]%Qp (tblockR ty q).
+    Observe [| cqp.frac q ≤ 1 |]%Qp (tblockR ty q).
   Proof.
     rewrite/tblockR=>-> ?. case_match; by apply _.
   Qed.
 
   #[global] Instance identityR_timeless cls mdc q : Timeless (identityR cls mdc q) := _.
-  #[global] Instance identityR_frac cls mdc : Fractional (identityR cls mdc) := _.
-  #[global] Instance identityR_as_frac cls mdc q : AsFractional (identityR cls mdc q) (identityR cls mdc) q := _.
+  #[global] Instance identityR_frac cls mdc c_q : Fractional (fun q => identityR cls mdc (cqp.mk c_q q)) := _.
+  #[global] Instance identityR_as_frac cls mdc c_q q :
+    AsFractional (identityR cls mdc (cqp.mk c_q q)) (fun q => identityR cls mdc (cqp.mk c_q q)) q.
+  Proof. by apply: Build_AsFractional. Qed.
   #[global] Instance identityR_strict_valid cls mdc q : Observe svalidR (identityR cls mdc q).
   Proof.
     red. eapply Rep_entails_at. intros.
