tests/const/const_test.v
@@ -21,13 +21,13 @@ Section with_Σ.
 
   Context `{Σ : cpp_logic}  {σ : genv.genv}.
 
-
+(*
   Definition CR := const_coreR (module := module) (Tnamed "_Z1C") 1.
   (* Eval hnf in CR. *)
 
   Definition DR := const_coreR (module := module) (Tnamed "_Z1D") 1.
   (* Eval hnf in DR. *)
-
+*)
 End with_Σ.
 
 
